move error bounds to new file

leapfrog_project/lf_harm_lemmas.v
@@ -17,37 +17,42 @@ Definition initial_t : float32 := 0.
 Definition half := Float32.div 1 2.
 
 Lemma half_repr : Float32.of_bits (Int.repr 1056964608) =  half.
-Proof. time prove_float_constants_equal. Qed.
+Proof. prove_float_constants_equal. Qed.
 
 Lemma neg1_repr: 
   Float32.neg (Float32.of_bits (Int.repr 1065353216)) = - (1).
 Proof.  prove_float_constants_equal. Qed. 
 
 Lemma exact_inverse_two: Float32.exact_inverse 2 = Some half.
-Proof.  prove_float_constants_equal. Time Qed.
+Proof.  prove_float_constants_equal. Qed.
+
 
 Lemma leapfrog_step_is_finite:
   forall n, 0 <= n < 100 ->
-          Binary.is_finite 24 128 (fst (Z.iter n leapfrog_step (initial_x, initial_v))) = true.
+    Binary.is_finite 24 128 (fst (Z.iter n leapfrog_step (initial_x, initial_v))) = true.
 Admitted.
 
-Definition leapfrog_stepx x v := fst (leapfrog_step (x,v)).
-Definition leapfrog_stepv x v := snd (leapfrog_step (x,v)).
+Definition leapfrog_stepx x v := fst (leapfrog_step' (x,v)).
+Definition leapfrog_stepv x v := snd (leapfrog_step' (x,v)).
 
 Import ListNotations.
 Definition _x : AST.ident := 1121%positive.
 Definition _v : AST.ident := 1117%positive.
 
+
 Import FPLangOpt. 
 Import FPLang.
 Import FPSolve.
 
-Definition e :=  ltac:(let e' := reify_float_expr constr:((float32_of_Z 1 / float32_of_Z 32)%F32 ) in exact e').
-Definition e1 := ltac:(let e' := HO_reify_float_expr constr:([_x; _v]) leapfrog_stepx in exact e').
-Definition e2 := ltac:(let e' := HO_reify_float_expr constr:([_x; _v]) leapfrog_stepv in exact e').
+
+Definition x' := ltac:(let e' := 
+  HO_reify_float_expr constr:([_x; _v]) leapfrog_stepx in exact e').
+Definition v' := ltac:(let e' := 
+  HO_reify_float_expr constr:([_x; _v]) leapfrog_stepv in exact e').
 
 
-Definition list_to_bound_env (bindings: list  (AST.ident * Test.varinfo)) (bindings2: list  (AST.ident * Values.val)) : (forall ty : type, AST.ident -> ftype ty) .
+Definition list_to_bound_env (bindings: list  (AST.ident * Test.varinfo)) 
+  (bindings2: list  (AST.ident * Values.val)) : (forall ty : type, AST.ident -> ftype ty) .
 pose (bm := Maps.PTree_Properties.of_list bindings).
 pose (vm := Maps.PTree_Properties.of_list bindings2). 
 intros ty i.
@@ -179,8 +184,8 @@ end.
 
 
 Definition leapfrog_bmap_list := 
-  [(_v, {|Test.var_type:=Tsingle; Test.var_name:=_v; Test.var_lobound:=powerRZ 2 (- 20); Test.var_hibound:=1|});
-  (_x,{|Test.var_type:=Tsingle; Test.var_name:=_x; Test.var_lobound:=powerRZ 2 (- 20); Test.var_hibound:=1|})].
+  [(_v, {|Test.var_type:=Tsingle; Test.var_name:=_v; Test.var_lobound:=-1; Test.var_hibound:=1|});
+  (_x,{|Test.var_type:=Tsingle; Test.var_name:=_x; Test.var_lobound:=-1; Test.var_hibound:=1|})].
 Definition leapfrog_vmap_list (x v : float32) := [(_x, Values.Vsingle x);(_v, Values.Vsingle v)].
 Definition leapfrog_env  := (fun x v => list_to_bound_env leapfrog_bmap_list (leapfrog_vmap_list x v)). 
 Definition leapfrog_bmap :=  Maps.PTree_Properties.of_list leapfrog_bmap_list.
@@ -191,53 +196,37 @@ Import B_Float_Notations.
 
 Lemma env_fval_reify_correct_leapfrog_step_x:
   forall x v : float32,
-  fval (leapfrog_env x v) e1 = leapfrog_stepx x v.
+  fval (leapfrog_env x v) x' = leapfrog_stepx x v.
 Proof.
 intros. 
-Time unfold_reflect' e1.  (* 0.045 sec *)
-Time unfold_float_ops_for_equality. (* 0.008 sec *)
-Time reflexivity. (* 0.000 sec *)
-Time Qed.  (* 0.013 sec *)
+unfold_reflect' x'.  
+unfold_float_ops_for_equality. 
+reflexivity.
+Qed.  
 
 
 Lemma env_fval_reify_correct_leapfrog_step_v:
   forall x v : float32,
-  fval (leapfrog_env x v) e2 = leapfrog_stepv x v.
+  fval (leapfrog_env  x v) v' = leapfrog_stepv x v.
 Proof.
 intros.
-Time unfold_reflect' e2.  (* 0.076 sec *)
-Time unfold_float_ops_for_equality. (* 0.0011 sec *)
-Time reflexivity. (* 0.001 sec *)
-Time Qed.  (* 0.03 sec *)
+unfold_reflect' v'.  
+unfold_float_ops_for_equality. 
+reflexivity. 
+Qed.  
 
 Lemma env_fval_reify_correct_leapfrog_step:
   forall x v : float32,
-  fval (leapfrog_env x v) e1 = leapfrog_stepx x v /\
-  fval (leapfrog_env x v) e2 = leapfrog_stepv x v.
+  fval (leapfrog_env x v) x' = leapfrog_stepx x v /\
+  fval (leapfrog_env  x v) v' = leapfrog_stepv x v.
 Proof.
 intros. 
 unfold leapfrog_env.
 unfold leapfrog_env; split.
-- unfold_reflect' e1. unfold_float_ops_for_equality. reflexivity.
-- unfold_reflect' e2. unfold_float_ops_for_equality. reflexivity.
+- unfold_reflect' x'. unfold_float_ops_for_equality. reflexivity.
+- unfold_reflect' v'. unfold_float_ops_for_equality. reflexivity.
 Qed.
 
-Lemma reify_correct_leapfrog_step:
-  forall x v : float32,
-  fval (list_to_env [(_x, Values.Vsingle x);(_v, Values.Vsingle v)]) e1 = leapfrog_stepx x v /\
-  fval (list_to_env [(_x, Values.Vsingle x);(_v, Values.Vsingle v)]) e2 = leapfrog_stepv x v.
-Proof.
-intros.
-unfold_reflect e1.
-unfold_reflect e2.
-split.
-all: try reflexivity.
-Admitted.  (* This Qed blows up.  The solution may be, 
-  in part, to replace the unfold_reflect  in vcfloat.v with the unfold_reflect' in this file,
-  and use it as in the proof of env_fval_reify_correct_leapfrog_step. 
-  But that's not the entire answer, becuse perhaps this list_to_env thing is 
-  obsolete now anyway?
-*)
 
 Ltac unfold_reflect_rval E := 
 match goal with |- context [rval (list_to_bound_env ?L1 ?L2) E] =>
@@ -269,21 +258,20 @@ Lemma env_rval_reify_correct_leapfrog_stepx:
   forall x1 v1 : R,
   x1 = B2R _ _ x ->
   v1 = B2R _ _ v -> 
-  rval (leapfrog_env x v) (optimize_div e1) = fst (leapfrog_stepR (x1,v1)).
+  rval (leapfrog_env x v) (optimize_div x') = fst (leapfrog_stepR (x1,v1)).
 Proof.
 intros.
 unfold leapfrog_env.
 match goal with |- context [rval ?env ?e] =>
   simplify_shift_div_opt e
-end.
+end. 
 match goal with |- context [rval ?env ?e] =>
   unfold_reflect_rval e; cbv [id]
 end.
-simpl; rewrite ?Z.pow_pos_fold. 
-unfold leapfrog_stepR, F, h, fst; subst.  
-replace (B2R (fprec Tsingle) 128 x) with (B2R 24 128 x) by auto.
-replace (B2R (fprec Tsingle) 128 v) with (B2R 24 128 v) by auto.
-all: try nra. 
+unfold leapfrog_stepR, F, h, fst, snd; subst.
+replace (B2R (fprec Tsingle) (femax Tsingle) x) with (B2R 24 128 x) by auto.
+replace (B2R (fprec Tsingle) (femax Tsingle) v) with (B2R 24 128 v) by auto.
+all: repeat f_equal; simpl; unfold Defs.F2R; simpl; nra.
 Qed.
 
 Lemma env_rval_reify_correct_leapfrog_stepv:
@@ -291,7 +279,7 @@ Lemma env_rval_reify_correct_leapfrog_stepv:
   forall x1 v1 : R,
   x1 = B2R _ _ x ->
   v1 = B2R _ _ v -> 
-  rval (leapfrog_env x v) (optimize_div e2) = snd (leapfrog_stepR (x1,v1)).
+  rval (leapfrog_env x v) (optimize_div v') = snd (leapfrog_stepR (x1,v1)).
 Proof.
 intros.
 unfold leapfrog_env.
@@ -303,10 +291,11 @@ match goal with |- context [rval ?env ?e] =>
 end.
 simpl; rewrite ?Z.pow_pos_fold. 
 unfold leapfrog_stepR, F, h, fst; subst.  
-replace (B2R (fprec Tsingle) 128 x) with (B2R 24 128 x) by auto.
-replace (B2R (fprec Tsingle) 128 v) with (B2R 24 128 v) by auto.
-all: try nra. 
+replace (B2R (fprec Tsingle) (femax Tsingle) x) with (B2R 24 128 x) by auto.
+replace (B2R (fprec Tsingle) (femax Tsingle) v) with (B2R 24 128 v) by auto.
+all: repeat f_equal; simpl; unfold Defs.F2R; simpl; nra.
 Qed.
+
 
 Import vcfloat.Test.
 
@@ -392,7 +381,35 @@ end
 
 Import Interval.Tactic.
 
-Ltac solve_one_cond2 var1 var2 := 
+
+Lemma neg_powerRZ (x:R) (n:Z) :
+  x <> R0 -> 
+  1 / (powerRZ x%R n%Z) = (powerRZ x%R (-n)%Z) .
+Proof.
+intros; pose proof power_RZ_inv x n H; symmetry; rewrite <- H0; nra. 
+Qed.
+
+Lemma mul_hlf_powerRZ (n:Z) :
+ / 2 * / powerRZ 2 n = powerRZ 2 (-n-1).
+Proof.
+assert (2 <> R0) by nra.
+replace (/ 2) with (1/2) by nra.
+replace (1 / 2 * / powerRZ 2 n) with
+(1 / 2 * powerRZ 2 (- n)).
+match goal with |- ?s = powerRZ ?a ?b' =>
+replace b' with (-1 + - n)%Z by ring
+end.
+pose proof powerRZ_add 2 (-1) (-n) H. rewrite H0.
+replace (1 / 2) with (powerRZ 2 (-1)). reflexivity.
+simpl; nra.
+replace (powerRZ 2 (- n)) with 
+(1 / powerRZ 2 n). 
+nra.
+(apply neg_powerRZ); nra.
+Qed.
+
+
+Ltac solve_one_cond2 := 
 match goal with |- eval_cond2 (mk_env ?bmap ?vmap) _ _ =>
  hnf;
  repeat
@@ -404,7 +421,10 @@ match goal with |- eval_cond2 (mk_env ?bmap ?vmap) _ _ =>
  repeat 
   (let H := fresh in intros ? H;
    simpl in H; cbv beta iota delta [error_bound Tsingle Tdouble fprec] in H;
-   simpl in H);
+simpl in H;
+rewrite ?IZR_Zpower_pos in H;
+rewrite ?mul_hlf_powerRZ in H);
+
  match goal with |- context [reval _ _ (mget ?M)] =>
    let m := fresh "m" in set (m:=M); compute in m;
     unfold reval;
@@ -419,43 +439,17 @@ match goal with |- eval_cond2 (mk_env ?bmap ?vmap) _ _ =>
    rewrite <- ?powerRZ_add in * by lra;
    simpl Z.add ;
 repeat
-  match goal with |- context [mk_env bmap ?vmap ?ty ?v'] =>
-       match goal with H: Maps.PTree.get ?v vmap = _ |- _ =>
-         change (mk_env bmap vmap ty v') with (mk_env bmap vmap ty v);
-         let x := fresh "x" in set (x := mk_env _ vmap _ v); 
+  match goal with |- context [mk_env ?bmap' ?vmap' ?ty ?v'] =>
+       match goal with H: Maps.PTree.get ?v vmap' = _ |- _ =>
+         change (mk_env bmap' vmap' ty v') with (mk_env bmap' vmap' ty v);
+         let x := fresh "x" in set (x := mk_env _ vmap' _ v); 
          hnf in x;
              compute in x; subst x; 
          try (cbv in H; inversion H; clear H; subst)
   end end; 
  repeat change (B2R (fprec ?x) _) with (FT2R x);
  try apply lesseq_less_or_eq;
- rewrite ?Rmult_1_l;
-try interval;
-try interval with (i_bisect var1, i_bisect var2, i_taylor var1, i_taylor var2)
-end.
-
-Ltac leapfrog_conds2_hold ex x v:=
-  match goal with 
-    H0: boundsmap_denote ?bmap ?vmap 
-      |- _ =>
-      apply boundsmap_denote_e in H0;
-      rewrite ?list_forall_Forall in *;
-      rewrite list_forall_Forall in H0;
-      rndval_replace; subst;
-      prepare_assumptions_about_free_variables;
-
-match goal with |- List.Forall (eval_cond2 _ ?M) _ =>
-   let m := fresh "m" in set (m:=M); compute in m; subst m;
-  fold Tsingle; fold Tdouble
-end;
-repeat
-    match goal with |- context [ type_lub ?a ?b ] =>
-     first [change (type_lub a b) with Tsingle 
-            |change (type_lub a b) with Tdouble]
-    end;
-
-repeat (apply List.Forall_cons; try apply List.Forall_nil;
-try solve_one_cond2 x v)
+ rewrite ?Rmult_1_l
 end.
 
 Ltac get_conds2 :=
@@ -526,31 +520,56 @@ Proof.
 intros; symmetry; apply powerRZ_pos_sub; auto. Qed.
 
 
-Lemma neg_powerRZ (x:R) (n:Z) :
-  x <> R0 -> 
-  1 / (powerRZ x%R n%Z) = (powerRZ x%R (-n)%Z) .
+Lemma mul_powerRZ (a:R) (n:Z) :
+ a / powerRZ 2 n = a * powerRZ 2 (-n).
 Proof.
-intros; pose proof power_RZ_inv x n H; symmetry; rewrite <- H0; nra. 
+replace (powerRZ 2 (- n)) with 
+(1 / powerRZ 2 n). 
+nra.
+(apply neg_powerRZ); nra.
 Qed.
 
 
 Ltac get_eps_delts := 
-match goal with 
-  H0: enum_exists 0
-       _ _ _|- _ =>
-hnf in H0; 
-repeat (let B := fresh "B" in destruct H0 as [?ed [B H0]]; simpl in B; 
-match type of B with context [error_bound _ ?a] => 
-  match a with 
-    |Normal   => (let d:= fresh "del" in (rename ed into d)) 
-    |Denormal => (let e:= fresh "eps" in (rename ed into e))
-  end
-end; unfold error_bound in B;
-  rewrite ?type_lub_id; simpl in B; 
-  rewrite ?IZR_Zpower_pos in B; 
-  rewrite ?neg_powerRZ
+match goal with
+  | H0:enum_exists 0 _ _ _
+    |- _ =>
+        hnf in H0;
+repeat match type of H0 with context [@mget ?a ?b ?c ?d ?e ?f] => 
+        let x := fresh "x" in set (x := @mget a b c d e f) in H0;
+compute in x; subst x
+   end; 
+repeat
+(let ed := fresh "ed" in
+let B := fresh "B" in
+destruct H0 as (ed & B & H0);
+            match type of B with
+            | context [ error_bound _ ?a ] =>
+                match a with
+                | Normal => let d := fresh "del" in
+                            rename
+                            ed into d
+                | Denormal => let e := fresh "eps" in
+                              rename
+                              ed into e
+                | uNormal => let e := fresh "eps" in
+                              rename
+                              ed into e
+                end
+             end;
+unfold error_bound in B; simpl in B;
+rewrite ?IZR_Zpower_pos in B;
+rewrite ?mul_hlf_powerRZ in B
 )
-end.
+end;
+repeat match goal with
+  | H0:Rabs ?e <= powerRZ 2 (-?x - ?y)
+    |- _ =>
+match type of H0 with context [Rabs ?e <= powerRZ 2 (-?x - ?y)] => 
+set (gg:=(-x - y)%Z) in H0; simpl in gg; subst gg
+end
+end
+.
 
 
 Ltac get_rexp_with_eps_delt e :=
@@ -567,16 +586,19 @@ Require Import Coq.Logic.FunctionalExtensionality.
 
 Lemma lf_env_eq: 
   forall x v : float32,
-boundsmap_denote leapfrog_bmap (leapfrog_vmap x v) ->
+boundsmap_denote leapfrog_bmap  (leapfrog_vmap x v) ->
 leapfrog_env x v = env_ (leapfrog_vmap x v).
 Proof.
-intros. pose proof (env_mk_env leapfrog_bmap (leapfrog_vmap x v) H). 
-replace (env_ (leapfrog_vmap x v)) with (mk_env leapfrog_bmap (leapfrog_vmap x v)). 
+intros. pose proof (env_mk_env (leapfrog_bmap ) (leapfrog_vmap x v) H). 
+replace (env_ (leapfrog_vmap x v)) with 
+  (mk_env (leapfrog_bmap ) (leapfrog_vmap x v)). 
 unfold leapfrog_env, list_to_bound_env, mk_env, leapfrog_bmap, leapfrog_vmap.
 apply functional_extensionality_dep; intro ty.
 apply functional_extensionality; intro i.
- destruct (Maps.PTree.get i (Maps.PTree_Properties.of_list leapfrog_bmap_list)) as [[t i' lo hi]|],
-    (Maps.PTree.get i (Maps.PTree_Properties.of_list (leapfrog_vmap_list x v))) as [v'|]; try contradiction; auto.
+ destruct (Maps.PTree.get i (Maps.PTree_Properties.of_list 
+    (leapfrog_bmap_list))) as [[t i' lo hi]|],
+    (Maps.PTree.get i (Maps.PTree_Properties.of_list (leapfrog_vmap_list x v))) 
+    as [v'|]; try contradiction; auto.
 Qed.
 
 
@@ -727,259 +749,180 @@ Proof.
 intros; field_simplify; reflexivity.
 Qed.
 
+Lemma Rabs_le_inv2 (x y :  R):
+0 <= Rabs x <= y -> - y <= x <= y.
+Proof.
+intros.
+assert (Rabs x <= y) by nra;
+pose proof Rabs_le_inv x y H0; assumption.
+Qed.
+
+
 Lemma leapfrog_stepx_is_finite:
   forall x v : float32,
-  boundsmap_denote leapfrog_bmap (leapfrog_vmap x v)->
-  Binary.is_finite _ _(fval (leapfrog_env x v) e1) = true.
-Proof. 
-intros.
+  boundsmap_denote leapfrog_bmap  (leapfrog_vmap x v)->
+  Binary.is_finite _ _(fval (leapfrog_env x v) x') = true.
+Proof.
+unfold optimize_div. 
+intros; subst.
 set (bmap:= leapfrog_bmap) in *.
 hnf in bmap. simpl in bmap.
-get_rndval_with_conds e1.
+get_rndval_with_conds x'.
 get_conds2.
 repeat (apply List.Forall_cons; try apply List.Forall_nil;
-try solve_one_cond2 (FT2R Tsingle val_x ) (FT2R Tsingle val_v )). 
-get_rndval_with_cond_correct e1 H0 H1 rndval s p.
+try solve_one_cond2; 
+try interval;
+try interval with (i_bisect (FT2R Tsingle val_v), 
+i_bisect (FT2R Tsingle val_x), i_taylor (FT2R Tsingle val_v), 
+i_taylor (FT2R Tsingle val_x))
+). 
+get_rndval_with_cond_correct x' H0 H1 rndval s p.
 replace (leapfrog_env x v) with (env_ (leapfrog_vmap x v)). 
-+ apply e0.
++ apply e.
 + symmetry; apply lf_env_eq; apply H.
 Qed.
 
 Lemma leapfrog_stepv_is_finite:
   forall x v : float32,
   boundsmap_denote leapfrog_bmap (leapfrog_vmap x v)->
-  Binary.is_finite _ _(fval (leapfrog_env x v) e2) = true.
+  Binary.is_finite _ _(fval (leapfrog_env  x v) v') = true.
 Proof. 
-intros.
+intros; subst.
 set (bmap:= leapfrog_bmap) in *.
 hnf in bmap. simpl in bmap.
-get_rndval_with_conds e2.
+get_rndval_with_conds v'.
 get_conds2.
 repeat (apply List.Forall_cons; try apply List.Forall_nil;
+try solve_one_cond2; 
+try interval;
+try interval with (i_bisect (FT2R Tsingle val_v), 
+i_bisect (FT2R Tsingle val_x), i_taylor (FT2R Tsingle val_v), 
+i_taylor (FT2R Tsingle val_x))
+). 
+repeat (apply List.Forall_cons; try apply List.Forall_nil;
 try solve_one_cond2 (FT2R Tsingle val_x ) (FT2R Tsingle val_v )). 
-get_rndval_with_cond_correct e2 H0 H1 rndval s p.
-replace (leapfrog_env x v) with (env_ (leapfrog_vmap x v)). 
-+ apply e0.
+get_rndval_with_cond_correct v' H0 H1 rndval s p.
+replace (leapfrog_env  x v) with (env_ (leapfrog_vmap x v)). 
++ apply e.
 + symmetry; apply lf_env_eq; apply H.
 Qed.
 
 Lemma leapfrog_stepx_not_nan:
   forall x v : float32,
   boundsmap_denote leapfrog_bmap (leapfrog_vmap x v)->
-  Binary.is_nan _ _(fval (leapfrog_env x v) e1) = false.
+  Binary.is_nan _ _(fval (leapfrog_env x v) x') = false.
 Proof. 
-intros.
+intros; subst;
 apply is_finite_not_is_nan.
-apply leapfrog_stepx_is_finite; apply H.
+apply leapfrog_stepx_is_finite; auto. 
 Qed.
 
 Lemma leapfrog_stepv_not_nan:
   forall x v : float32,
   boundsmap_denote leapfrog_bmap (leapfrog_vmap x v)->
-  Binary.is_nan _ _(fval (leapfrog_env x v) e2) = false.
+  Binary.is_nan _ _(fval (leapfrog_env x v) v') = false.
 Proof. 
-intros.
+intros; subst;
 apply is_finite_not_is_nan.
-apply leapfrog_stepv_is_finite; apply H.
+apply leapfrog_stepv_is_finite; auto. 
 Qed.
 
 Lemma leapfrog_opt_stepx_is_finite:
   forall x v : float32,
   boundsmap_denote leapfrog_bmap (leapfrog_vmap x v)->
-  Binary.is_finite _ _ (fval (leapfrog_env x v) (optimize_div e1)) = true.
+  Binary.is_finite _ _ (fval (leapfrog_env x v) (optimize_div x')) = true.
 Proof.
 intros.
-set (env:=(leapfrog_env x v)) in *.
+set (env:=(leapfrog_env x v)) in *. 
 pose proof 
-  binary_float_eqb_is_finite (fval env e1) 
-    (fval env (optimize_div e1)) 
-    (leapfrog_stepx_is_finite x v H) 
-    (optimize_div_correct' env e1 (leapfrog_stepx_not_nan x v H)).
+  (optimize_div_correct' env x' (leapfrog_stepx_not_nan x v H )).
+pose proof 
+  binary_float_eqb_is_finite (fval env x') 
+    (fval env (optimize_div x'))
+    (leapfrog_stepx_is_finite x v H) H0.
 assumption.
 Qed.
 
 Lemma leapfrog_opt_stepv_is_finite:
   forall x v : float32,
   boundsmap_denote leapfrog_bmap (leapfrog_vmap x v)->
-  Binary.is_finite _ _ (fval (leapfrog_env x v) (optimize_div e2)) = true.
+  Binary.is_finite _ _ (fval (leapfrog_env  x v) (optimize_div v')) = true.
 Proof.
 intros.
 set (env:=(leapfrog_env x v)) in *.
 pose proof 
-  binary_float_eqb_is_finite (fval env e2) 
-    (fval env (optimize_div e2)) 
-    (leapfrog_stepv_is_finite x v H) 
-    (optimize_div_correct' env e2 (leapfrog_stepv_not_nan x v H)).
+  binary_float_eqb_is_finite (fval env v') 
+    (fval env (optimize_div v')) 
+    (leapfrog_stepv_is_finite x v H)
+    (optimize_div_correct' env v' (leapfrog_stepv_not_nan x v H)).
 assumption.
 Qed.
 
-
-(* single step velocity error *)
-Lemma one_step_errorv:
-  forall x v : float32,
-    boundsmap_denote leapfrog_bmap (leapfrog_vmap x v)->
-    Rle (Rabs (Rminus (rval (leapfrog_env x v) (optimize_div e2)) 
-    (B2R _ _ (fval (leapfrog_env x v) (optimize_div e2))))) 
-         (4934642575282197 / 75557863725914323419136)%R.
+Lemma error_reduce a b c d :
+a - (b * (1 + c) + d) = 
+(a - b )  - b * c - d.
 Proof.
 intros.
-set (bmap:= leapfrog_bmap) in *.
-hnf in bmap. simpl in bmap.
-match goal with |- context [ rval ?env ?e] =>
-simplify_shift_div_opt e
-end.
-match goal with |- context [ rval ?env ?e] =>
-get_rndval_with_conds e
-end.
-get_conds2.
-repeat (apply List.Forall_cons; try apply List.Forall_nil;
-try solve_one_cond2 (FT2R Tsingle val_x ) (FT2R Tsingle val_v )). 
-match goal with |- context [ rval ?env ?e] =>
-get_rndval_with_cond_correct e H0 H1 rndval s p;
-set (ty:= type_of_expr e) in *;
-simpl in ty;
-cbv [Datatypes.id] in ty;   
-repeat change (type_lub Tsingle Tsingle) with Tsingle in ty; 
-unfold ty in *; clear ty
-end.
-(* Populate hyps with some bounds on x and v*)
-fv_prepare_assumptions.
-(* turn rndval rexp to flt with eps delt *)
-rndval_replace.
-subst si2 s r;
-get_eps_delts.
-clear correct.
-revert e3; reduce_abs_error.
-(* env rewrite *)
-replace ((env_ (leapfrog_vmap val_x val_v))) with (leapfrog_env val_x val_v) in * by
-(apply lf_env_eq; apply BMD).
-(* var rewrites *)
-replace (leapfrog_env val_x val_v Tsingle lf_harm_lemmas._x) with val_x in * by 
-(cbv in Hval_x;inversion Hval_x; clear Hval_x; subst; auto).
-replace (leapfrog_env val_x val_v Tsingle lf_harm_lemmas._v) with val_v in * by 
-(cbv in Hval_v;inversion Hval_v; clear Hval_v; subst; auto).
-change (fprec Tsingle) with 24%Z in *; 
-change (femax Tsingle) with 128%Z in *.
-intros. rewrite <- e3.
-match goal with |- context[ (?v + ?b * ?c - ((?v + ?b * ?c') * (1 + ?del) + ?eps))] =>
-pose proof (del_eps_reduce2 1 v (b*c) (b*c') del eps) as uH;
-rewrite ?Rmult_1_l in uH;
-rewrite uH; clear uH
-end.
-
-
-match goal with |- context[
-  ?a * (?b * ( - ?c + ?d)) -
-  ?a * (?b * ((- ?c + ?d') * (1 + ?del0) + ?eps0)) ] =>
-replace 
-(a * (b * ( - c + d)) - a * (b * ((- c + d') * (1 + del0) + eps0)))
-with
-(a*b*(d - d') - a*b*(- c + d')*del0 - a*b* eps0) by 
-( pose proof (del_eps_reduce2 (a*b) (-c) (d) (d') del0 eps0) as uH;
-try rewrite <- uH; try field_simplify; try reflexivity)
-end.
-
-match goal with |- context [
-(-(?a + ?B + ?D) - - 
-(((?a + ?B ) * (1 + ?del2) + ?eps2 + ?D) * (1 + ?del1) + ?eps1))] =>
-replace 
-(-(a + B + D) - - 
-(((a + B ) * (1 + del2) + eps2 + D) * (1 + del1) + eps1))
-with
-(-(a + B + D) + 
-(((a + B ) * (1 + del2) + eps2 + D) * (1 + del1) + eps1))
-by (field_simplify; try reflexivity);
-replace 
-(-(a + B + D) + 
-(((a + B ) * (1 + del2) + eps2 + D) * (1 + del1) + eps1)) with
-((a+B)*del2 + eps2 + (a+B+D+(a+B)*del2 + eps2)*del1 +eps1) 
-by (field_simplify; try reflexivity)
-end.
-
-repeat match goal with |- context [?a * (?b + ?c)] =>
-    rewrite ?Rmult_plus_distr_l; rewrite ?Rmult_plus_distr_r
-end; rewrite ?Rmult_1_r.
-match goal with |- context [Rabs (?v) <= _] =>
-try interval_intro (Rabs v);
-try interval;
-try nra
-end.
+nra.
 Qed.
 
-Definition error_v:= (4934642575282197 / 75557863725914323419136).
 
-(* single step position error *)
-Lemma one_step_errorx:
+Definition iternF  (n:nat) (x v :float32) :=  leapfrog' (x%F32, v%F32) n.
+Definition iternR (n:nat) (x v :R) :=  leapfrogR (x,v) n .
+
+Lemma step_iternR : 
+  forall n : nat,
+  forall x v : R,
+  (iternR (S n) x v) = leapfrog_stepR (iternR n x v).
+Proof.
+intros; unfold iternR; 
+rewrite ?lfn_eq_lfstepR; 
+congruence.
+Qed.
+
+Lemma step_iternF : 
+  forall n : nat,
   forall x v : float32,
-    boundsmap_denote leapfrog_bmap (leapfrog_vmap x v)->
-    Rle (Rabs (Rminus (rval (leapfrog_env x v) (optimize_div e1)) 
-   (B2R _ _ (fval (leapfrog_env x v) (optimize_div e1))))) 
-         (4719104053608481 / 37778931862957161709568)%R.
+  (iternF (S n) x v) = leapfrog_step' (iternF n x v).
+Proof.
+intros; unfold iternF; 
+rewrite ?lfn_eq_lfstep; 
+congruence.
+Qed.
+
+Lemma Rabs_triang_aux : 
+  forall a b c : R,
+  Rabs a + Rabs b <= c ->
+  Rabs( a + b ) <= c.
 Proof.
 intros.
-set (bmap:= leapfrog_bmap) in *.
-hnf in bmap. simpl in bmap.
-match goal with |- context [ rval ?env ?e] =>
-simplify_shift_div_opt e
-end.
-
-match goal with |- context [ rval ?env ?e] =>
-get_rndval_with_conds e
-end.
-
-get_conds2.
-
-repeat (apply List.Forall_cons; try apply List.Forall_nil;
-try solve_one_cond2 (FT2R Tsingle val_x ) (FT2R Tsingle val_v )). 
-
-
-match goal with |- context [ rval ?env ?e] =>
-get_rndval_with_cond_correct e H0 H1 rndval s p;
-set (ty:= type_of_expr e) in *;
-simpl in ty;
-cbv [Datatypes.id] in ty;   
-repeat change (type_lub Tsingle Tsingle) with Tsingle in ty; 
-unfold ty in *; clear ty
-end.
-
-(* Populate hyps with some bounds on x and v*)
-fv_prepare_assumptions.
-(* turn rndval rexp to flt with eps delt *)
-rndval_replace.
-subst si2 s r;
-get_eps_delts.
-clear correct.
-revert e3; reduce_abs_error.
-
-(* env rewrite*)
-replace ((env_ (leapfrog_vmap val_x val_v))) with (leapfrog_env val_x val_v) in * by
-(apply lf_env_eq; apply BMD).
-(* var rewrites *)
-replace (leapfrog_env val_x val_v Tsingle lf_harm_lemmas._x) with val_x in * by 
-(cbv in Hval_x;inversion Hval_x; clear Hval_x; subst; auto).
-replace (leapfrog_env val_x val_v Tsingle lf_harm_lemmas._v) with val_v in * by 
-(cbv in Hval_v;inversion Hval_v; clear Hval_v; subst; auto).
-
-change (fprec Tsingle) with 24%Z in *; 
-change (femax Tsingle) with 128%Z in *. 
-
-intros; rewrite <- e3.
-
-repeat match goal with |- context [?a * (?b + ?c)] =>
-    rewrite ?Rmult_plus_distr_l; rewrite ?Rmult_plus_distr_r
-end ; rewrite ?Rmult_1_r;
-match goal with |- context [Rabs (?a + ?b + ?c -(?v)) <= _] =>
-field_simplify (a + b + c - (v))
-end;
-match goal with |- context [Rabs (?v) <= _] =>
-field_simplify v;
-interval_intro (Rabs v);
-try interval
-end.
+pose proof Rabs_triang a b.
+pose proof Rle_trans _ _ _ H0 H; assumption.
 Qed.
 
-Definition error_x :=  (4719104053608481 / 37778931862957161709568).
 
+Lemma Rabs_triang_aux2 : 
+  forall a b c d : R,
+  Rabs a + Rabs b + Rabs c <= d ->
+  Rabs (a + b) + Rabs c <= d.
+Proof.
+intros.
+assert (Rabs (a + b) + Rabs c <= Rabs a + Rabs b + Rabs c).
+pose proof Rcomplements.Rle_minus_r 
+  (Rabs (a + b)) (Rabs a + Rabs b + Rabs c) (Rabs c); destruct H0. 
+try apply H0; field_simplify; apply Rabs_triang.
+try pose proof Rle_trans _ _ d H0 H; assumption.
+Qed.
+
+Lemma Rabs_triang_aux3 : 
+  forall a b c x y z : R,
+  Rabs a <= x ->
+  Rabs b <= y ->
+  Rabs c <= z ->
+  Rabs a + Rabs b + Rabs c <= x + y +z.
+Proof. intros; nra. Qed.
+
+(*
 Lemma local_error_x :
   forall x v : float32,
   forall x1 v1 : R,
@@ -1032,186 +975,7 @@ apply binary_float_eqb_eq in H2; subst; reflexivity.
 + rewrite (@env_rval_reify_correct_leapfrog_stepv x v x1 v1); auto.
 Qed.
 
-
-Definition iternF  (n:nat) (x v :float32) :=  leapfrog (x%F32, v%F32) n.
-Definition iternR (n:nat) (x v :R) :=  leapfrogR (x,v) n .
-
-Lemma step_iternR : 
-  forall n : nat,
-  forall x v : R,
-  (iternR (S n) x v) = leapfrog_stepR (iternR n x v).
-Proof.
-intros; unfold iternR; 
-rewrite ?lfn_eq_lfstepR; 
-congruence.
-Qed.
-
-Lemma step_iternF : 
-  forall n : nat,
-  forall x v : float32,
-  (iternF (S n) x v) = leapfrog_step (iternF n x v).
-Proof.
-intros; unfold iternF; 
-rewrite ?lfn_eq_lfstep; 
-congruence.
-Qed.
-
-Lemma Rabs_triang_aux : 
-  forall a b c : R,
-  Rabs a + Rabs b <= c ->
-  Rabs( a + b ) <= c.
-Proof.
-intros.
-pose proof Rabs_triang a b.
-pose proof Rle_trans _ _ _ H0 H; assumption.
-Qed.
+*)
 
 
-Lemma Rabs_triang_aux2 : 
-  forall a b c d : R,
-  Rabs a + Rabs b + Rabs c <= d ->
-  Rabs (a + b) + Rabs c <= d.
-Proof.
-intros.
-assert (Rabs (a + b) + Rabs c <= Rabs a + Rabs b + Rabs c).
-pose proof Rcomplements.Rle_minus_r 
-  (Rabs (a + b)) (Rabs a + Rabs b + Rabs c) (Rabs c); destruct H0. 
-try apply H0; field_simplify; apply Rabs_triang.
-try pose proof Rle_trans _ _ d H0 H; assumption.
-Qed.
-
-Lemma Rabs_triang_aux3 : 
-  forall a b c x y z : R,
-  Rabs a <= x ->
-  Rabs b <= y ->
-  Rabs c <= z ->
-  Rabs a + Rabs b + Rabs c <= x + y +z.
-Proof. intros; nra. Qed.
-
-Lemma global_error_x_aux : 
-  forall x v : float32,
-  forall x' v' x'' v'' a b : R,
-  boundsmap_denote leapfrog_bmap (leapfrog_vmap x v)->
-  x' = B2R _ _ x -> v' = B2R _ _ v ->
-  Rabs(x'' - x') <= a -> Rabs(v'' - v') <= b ->
-  Rabs( fst (leapfrog_stepR (x'',v'')) - B2R _ _ (fst (leapfrog_step (x,v)) )) <=
-  ((1 - 0.5 * (pow lf_harm_real.h 2)) * a + (lf_harm_real.h) * b + error_x). 
-Proof. 
-intros.
-match goal with |- context [Rabs(?x1 -?x3) <= ?c] =>
-  let x2:= constr:(fst(leapfrog_stepR (x',v'))) in
-  replace (Rabs(x1 - x3)) with (Rabs(x1 -x2 + x2 - x3)) by
-  (field_simplify (x1 - x2 + x2 - x3); nra);
-  set (aa:= (x1-x2));
-  replace (Rminus (aa + x2) x3) with (Rplus aa (x2- x3)) by nra;
-  set (bb:= (x2-x3));
-  try apply Rabs_triang_aux; unfold aa; unfold bb; clear aa bb
-end.
-rewrite ?one_stepR_x_alt2.
-apply Rabs_triang_aux2.
-fold (leapfrog_stepx x v).
-apply Rabs_triang_aux3.
-+ unfold fst, lf_harm_real.h. rewrite ?abs_mul; nra.
-+ unfold snd, lf_harm_real.h. rewrite ?abs_mul; nra.
-+ try apply local_error_x; auto.
-Qed.
-
-Lemma global_error_v_aux : 
-  forall x v : float32,
-  forall x' v' x'' v'' a b : R,
-  boundsmap_denote leapfrog_bmap (leapfrog_vmap x v)->
-  x' = B2R _ _ x -> v' = B2R _ _ v ->
-  Rabs(x'' - x') <= a -> Rabs(v'' - v') <= b ->
-  Rabs( snd (leapfrog_stepR (x'',v'')) - B2R _ _ (snd (leapfrog_step (x,v)) )) <=
-  ((1 - 0.5 * (pow lf_harm_real.h 2)) * b + 
-    (0.5 * (lf_harm_real.h) * (2 - 0.5 * (pow lf_harm_real.h 2 )) * a) + error_v). 
-Proof. 
-intros.
-match goal with |- context [Rabs(?x1 -?x3) <= ?c] =>
-  let x2:= constr:(snd(leapfrog_stepR (x',v'))) in
-  replace (Rabs(x1 - x3)) with (Rabs(x1 -x2 + x2 - x3)) by
-  (field_simplify (x1 - x2 + x2 - x3); nra);
-  set (aa:= (x1-x2));
-  replace (Rminus (aa + x2) x3) with (Rplus aa (x2- x3)) by nra;
-  set (bb:= (x2-x3));
-  try apply Rabs_triang_aux; unfold aa; unfold bb; clear aa bb
-end.
-rewrite ?one_stepR_v_alt2.
-apply Rabs_triang_aux2.
-fold (leapfrog_stepv x v).
-apply Rabs_triang_aux3.
-+ unfold snd, lf_harm_real.h; rewrite ?abs_mul; nra.
-+ unfold fst, lf_harm_real.h; rewrite ?Rabs_Ropp; rewrite ?abs_mul; nra.
-+ try apply local_error_v; auto.
-Qed.
-
-
-Lemma global_error:
-  forall x v : float32, 
-  (forall m: nat, 
-  forall x' v' : float32, 
-  (x',v') = (iternF m x%F32 v%F32) -> 
-  boundsmap_denote leapfrog_bmap (leapfrog_vmap x' v')) ->
-  forall n: nat, 
-  forall x1 v1 : R,
-  x1 = B2R _ _ x ->
-  v1 = B2R _ _ v -> 
-  INR n <= 0.5 * 1/lf_harm_real.h -> 
-  Rle (Rabs (Rminus (fst(iternR n x1%R v1%R)) (B2R _ _ (fst(iternF n x%F32 v%F32))))) 
-   (2*(pow lf_harm_real.h 3) * sqrt (INR n)) /\
-  Rle (Rabs (Rminus (snd(iternR n x1%R v1%R)) (B2R _ _ (snd(iternF n x%F32 v%F32))))) 
-  (2*(pow lf_harm_real.h 3) * sqrt (INR n)) .
-Proof.
-intros. 
-replace (0.5 * 1 / lf_harm_real.h) with 
-16 in H2 by (unfold lf_harm_real.h; nra).
-induction n.
-- unfold iternF ,iternR ,INR, leapfrog, leapfrogR, 
-leapfrog_stepx,lf_harm_real.h.
-unfold fst; unfold snd; subst.
-replace (B2R 24 128 x - B2R 24 128 x) with 0 by nra;
-replace (B2R 24 128 v - B2R 24 128 v) with 0 by nra.
-split. all: (rewrite ?sqrt_0; interval).
-- rewrite ?S_INR in H2.
-apply Rminus_plus_le_minus in H2; field_simplify in H2.
-assert (INR n <= 16) as Hn by nra.
-pose proof IHn Hn; clear IHn Hn;
-assert (INR n <= 15) as Hn by nra; clear H2.
-rewrite ?step_iternR; rewrite ?step_iternF. 
-try pose proof H n 
-  ((fst (iternF n x v))) ((snd (iternF n x v))); clear H. 
-destruct (iternR n x1 v1) as (xnr, vnr). 
-destruct (iternF n x v) as (xnf, vnf).
-unfold fst, snd in H2; pose proof H2 eq_refl; clear H2.
-unfold fst, snd in H3. 
-set (r_xnf:= B2R _ _ xnf ) in *; assert (r_xnf = B2R 24 128 xnf) by auto.
-set (r_vnf:= B2R _ _ vnf) in *;  assert (r_vnf = B2R 24 128 vnf) by auto.
-rewrite ?step_iternR; rewrite ?step_iternF. 
-set (a:= 2 * lf_harm_real.h ^ 3 * sqrt (INR n)).
-destruct H3 as (IHx & IHv); split.
-(* x case *)
-+ pose proof global_error_x_aux 
-  xnf vnf r_xnf r_vnf xnr vnr a a H H2 H4 IHx IHv.
-eapply Rle_trans. 
--- apply H3.
--- rewrite ?S_INR.
-unfold error_x, a, lf_harm_real.h in *.
-pose proof pos_INR n.
-apply Rminus_le.
-(* depth is necessary for sqrt? *)
-try interval with  
-(i_bisect (INR n), i_depth 15).
-(* v case *)
-+ pose proof global_error_v_aux 
-  xnf vnf r_xnf r_vnf xnr vnr a a H H2 H4 IHx IHv.
-eapply Rle_trans. 
--- apply H3.
--- rewrite ?S_INR.
-unfold error_v, a, lf_harm_real.h in *.
-pose proof pos_INR n.
-apply Rminus_le.
-(* depth is necessary for sqrt? *)
-try interval with  
-(i_bisect (INR n), i_depth 15).
-Qed.
 
